cleanup

Foundation/Modal/Formula.lean
@@ -338,26 +338,6 @@ instance : Encodable (Formula α) where
 
 end Encodable
 
-
-def letterless : Formula α → Prop
-  | atom _ => False
-  | ⊥ => True
-  | □φ => φ.letterless
-  | φ ➝ ψ => (φ.letterless) ∧ (ψ.letterless)
-
-namespace letterless
-
-variable {φ ψ : Formula α}
-
-@[simp] lemma not_atom : ¬(letterless (atom p)) := by simp [letterless]
-
-lemma def_imp : (φ ➝ ψ).letterless → φ.letterless ∧ ψ.letterless := by simp [letterless]
-lemma def_imp₁ : (φ ➝ ψ).letterless → φ.letterless := λ h => def_imp h |>.1
-lemma def_imp₂ : (φ ➝ ψ).letterless → ψ.letterless := λ h => def_imp h |>.2
-lemma def_box : (□φ).letterless → φ.letterless := by simp [letterless]
-
-end letterless
-
 end Formula
 
 end Modal
@@ -607,18 +587,6 @@ lemma Formula.subst.def_comp {s₁ s₂ : Substitution α} {φ : Formula α} : �
 
 class SubstitutionClosed (S : Set (Formula α)) where
   closed : ∀ φ ∈ S, (∀ s : Substitution α, φ⟦s⟧ ∈ S)
-
-
-def ZeroSubstitution (α) := {s : Substitution α // ∀ {a : α}, ((.atom a)⟦s⟧).letterless }
-
-lemma Formula.letterless_zeroSubst {φ : Formula α} {s : ZeroSubstitution α} : (φ⟦s.1⟧).letterless := by
-  induction φ <;> simp [Formula.letterless, *];
-  case hatom => exact s.2;
-
-lemma Formula.toModalFormula.letterless {φ : Propositional.Formula α} (h : φ.letterless) : φ.toModalFormula.letterless := by
-  induction φ using Propositional.Formula.rec' <;> simp_all [Propositional.Formula.letterless, Formula.letterless];
-
-instance : Coe (Propositional.ZeroSubstitution α) (Modal.ZeroSubstitution α) := ⟨λ ⟨s, p⟩ => ⟨λ φ => s φ, λ {_} => Formula.toModalFormula.letterless p⟩⟩
 
 end Substitution
 
