Foundation/Modal/Kripke/Rank.lean
@@ -1,0 +1,195 @@
+import Foundation.Modal.Kripke.Logic.GL.Tree
+import Foundation.Modal.Kripke.ExtendRoot
+
+namespace LO.Modal
+
+noncomputable section
+
+namespace Kripke
+
+variable {φ ψ : Formula ℕ}
+         {F : Frame} {r : F} [Fintype F] [F.IsTree r] {x y i j : F}
+
+def Frame.World.finHeight (i : F) : ℕ := fcwHeight (· ≺ ·) i
+
+def Frame.finHeight (F : Frame) {r : F} [Fintype F] [F.IsTree r] : ℕ := Frame.World.finHeight r
+
+namespace Frame
+
+lemma World.finHeight_lt_whole_finHeight {i : F} (hi : r ≺ i) :
+    Frame.World.finHeight i < F.finHeight := fcwHeight_gt_of hi
+
+lemma World.finHeight_le_whole_finHeight (i : F) :
+    Frame.World.finHeight i ≤ F.finHeight := by
+  by_cases hi : i = r
+  · rcases hi; rfl
+  · have : r ≺ i := root_genaretes'! i hi
+    exact le_of_lt (fcwHeight_gt_of this)
+
+lemma World.finHeight_lt_of_rel (hij : i ≺ j) : Frame.World.finHeight i > Frame.World.finHeight j := fcwHeight_gt_of hij
+
+lemma World.exists_of_lt_finHeight (hn : n < Frame.World.finHeight i) : ∃ j : F, i ≺ j ∧ Frame.World.finHeight j = n := fcwHeight_lt hn
+
+lemma finHeight_lt_iff_relItr {i : F} :
+    Frame.World.finHeight i < n ↔ ∀ j, ¬i ≺^[n] j  := by
+  match n with
+  |     0 => simp_all
+  | n + 1 =>
+    suffices Frame.World.finHeight i ≤ n ↔ ∀ j : F, i ≺ j → Frame.World.finHeight j < n by
+      calc
+        Frame.World.finHeight i < n + 1
+          ↔ Frame.World.finHeight i ≤ n := Nat.lt_add_one_iff
+        _ ↔ ∀ j, i ≺ j → Frame.World.finHeight j < n := this
+        _ ↔ ∀ j, i ≺ j → ∀ k, ¬j ≺^[n] k := by simp [finHeight_lt_iff_relItr (n := n)]
+        _ ↔ ∀ k j, i ≺ j → ¬j ≺^[n] k    := by grind
+        _ ↔ ∀ j, ¬i ≺^[n + 1] j  := by simp
+    constructor
+    · exact fun h j hij ↦ lt_of_lt_of_le (fcwHeight_gt_of hij) h
+    · exact fcwHeight_le
+
+lemma le_finHeight_iff_relItr {i : F} :
+    n ≤ Frame.World.finHeight i ↔ ∃ j, i ≺^[n] j := calc
+  n ≤ Frame.World.finHeight i ↔ ¬Frame.World.finHeight i < n := Iff.symm Nat.not_lt
+  _                           ↔ ∃ j, i ≺^[n] j := by simp [finHeight_lt_iff_relItr]
+
+lemma finHeight_eq_iff_relItr {i : F} :
+    Frame.World.finHeight i = n ↔ (∃ j, i ≺^[n] j) ∧ (∀ j, i ≺^[n] j → ∀ k, ¬j ≺ k) := calc
+  Frame.World.finHeight i = n
+    ↔ Frame.World.finHeight i < n + 1 ∧ n ≤ Frame.World.finHeight i := by simpa [Nat.lt_succ_iff] using Nat.eq_iff_le_and_ge
+  _ ↔ (∀ j, ¬i ≺^[n + 1] j) ∧ (∃ j, i ≺^[n] j) := by simp [finHeight_lt_iff_relItr, le_finHeight_iff_relItr]
+  _ ↔ (∀ k j, i ≺^[n] j → ¬j ≺ k) ∧ (∃ j, i ≺^[n] j) := by simp only [HRel.Iterate.forward, not_exists, not_and]
+  _ ↔ (∃ j, i ≺^[n] j) ∧ (∀ j, i ≺^[n] j → ∀ k, ¬j ≺ k) := by grind
+
+lemma exists_terminal (i : F) : ∃ j, i ≺^[Frame.World.finHeight i] j := le_finHeight_iff_relItr.mp (by simp)
+
+lemma eq_finHeight_root : Frame.World.finHeight x = F.finHeight ↔ x = r := by
+  constructor;
+  . rintro h;
+    contrapose! h;
+    apply Nat.ne_of_lt;
+    apply Frame.World.finHeight_lt_whole_finHeight;
+    apply F.root_genaretes'!;
+    assumption;
+  . tauto;
+
+lemma terminal_rel_finHeight (h : x ≺^[World.finHeight x] y) : ∀ z, ¬y ≺ z := by
+  intro z Ryz;
+  suffices World.finHeight x + 1 ≤ World.finHeight x by omega;
+  exact le_finHeight_iff_relItr.mpr ⟨z, HRel.Iterate.forward.mpr ⟨y, h, Ryz⟩⟩;
+
+namespace extendRoot
+
+@[simp] lemma finHeight_pos : 0 < (F.extendRoot 1).finHeight := by
+  apply lt_fcwHeight ?_ (by simp)
+  · exact Sum.inr r
+  trivial
+
+@[simp] lemma finHeight₁ : (F.extendRoot 1).finHeight = F.finHeight + 1 := by
+  let l := World.finHeight (extendRoot.root : F.extendRoot 1)
+  suffices
+      l ≤ Frame.World.finHeight r + 1 ∧
+      Frame.World.finHeight r < l by
+    simpa using Nat.eq_iff_le_and_ge.mpr this
+  constructor
+  · suffices l - 1 ≤ World.finHeight r from Nat.le_add_of_sub_le this
+    apply le_finHeight_iff_relItr.mpr
+    by_cases hl : l - 1 = 0
+    · exact ⟨r, by simp [hl]⟩
+    have lpos : 0 < l - 1 := Nat.zero_lt_of_ne_zero hl
+    have e : l = (l - 1) + 1 := by
+      symm; exact Nat.sub_add_cancel Frame.extendRoot.finHeight_pos
+    have : ∃ j, extendRoot.root ≺^[l] j := exists_terminal (extendRoot.root : F.extendRoot 1)
+    rcases this with ⟨j, hj⟩
+    have : ∃ z, extendRoot.root ≺ z ∧ z ≺^[l - 1] j := by
+      rw [e] at hj
+      simpa using hj
+    rcases this with ⟨z, hz, hzj⟩
+    have : ∃ x, j = embed x := eq_inr_of_root_rel <| HRel.Iterate.unwrap_of_trans_of_pos finHeight_pos hj
+    rcases this with ⟨j, rfl⟩
+    rcases not_root_of_from_root'₁ hz with (rfl | ⟨z, rfl, Rrz⟩)
+    · exact ⟨j, embed_rel_iterate_embed_iff_rel.mp hzj⟩
+    use j
+    exact HRel.Iterate.constant_trans_of_pos lpos Rrz (embed_rel_iterate_embed_iff_rel.mp hzj)
+  · suffices World.finHeight r + 1 ≤ World.finHeight extendRoot.root from this
+    apply le_finHeight_iff_relItr.mpr
+    rcases exists_terminal r with ⟨j, hj⟩
+    exact ⟨j, r, by trivial, embed_rel_iterate_embed_iff_rel.mpr hj⟩
+
+lemma eq_original_finHeight : Frame.World.finHeight (x : F.extendRoot 1) = Frame.World.finHeight x := by
+  apply finHeight_eq_iff_relItr.mpr;
+  constructor;
+  . obtain ⟨y, Rxy⟩ := exists_terminal (i := x);
+    use y;
+    apply extendRoot.embed_rel_iterate_embed_iff_rel.mpr;
+    exact Rxy;
+  . rintro (_ | y) Rxy (_ | z);
+    . simp;
+    . -- TODO: extract no loop lemma (x ≺^[n] i cannot happen where x is original and i is new elements by extension)
+      exfalso;
+      have : extendRoot.root ≺ (x : F.extendRoot 1) := Frame.root_genaretes'! (F := F.extendRoot 1) x (by simp);
+      have : (x : F.extendRoot 1) ≺ x :=
+        HRel.Iterate.unwrap_of_trans_of_pos (by omega) $
+        HRel.Iterate.comp (m := 1) |>.mp ⟨_, Rxy, by simpa⟩;
+      exact Frame.irrefl _ this;
+    . apply Frame.asymm;
+      exact Frame.root_genaretes'! (F := F.extendRoot 1) y (by simp);
+    . have := terminal_rel_finHeight $ extendRoot.embed_rel_iterate_embed_iff_rel.mp Rxy;
+      exact extendRoot.embed_rel_embed_iff_rel.not.mpr $ this z;
+
+lemma eq_original_finHeight_root : Frame.World.finHeight (r : F.extendRoot 1) = F.finHeight := eq_original_finHeight
+
+@[grind]
+lemma iff_eq_finHeight_eq_original_root {x : F.extendRoot 1} : Frame.World.finHeight x = F.finHeight ↔ x = r := by
+  constructor;
+  . rcases x with (a | x);
+    . intro h;
+      have := h ▸ finHeight₁ (F := F);
+      simp [Frame.finHeight] at this;
+    . intro h;
+      suffices x = r by simp [this];
+      apply Frame.eq_finHeight_root.mp;
+      exact h ▸ Frame.extendRoot.eq_original_finHeight.symm;
+  . rintro rfl;
+    exact eq_original_finHeight_root;
+
+end extendRoot
+
+
+namespace pointGenerate
+
+open Classical in
+instance [Fintype F] : Fintype (F↾x) := by apply Subtype.fintype;
+
+instance [F.IsTree r] : (F↾x).IsTree ⟨x, by tauto⟩ := by constructor;
+
+axiom eq_original_finHeight (hxy : y = x ∨ x ≺^+ y) : Frame.World.finHeight (F := F↾x) (⟨y, hxy⟩) = Frame.World.finHeight y
+
+end pointGenerate
+
+end Frame
+
+
+section
+
+variable {M : Model} {r : M.World} [M.IsFiniteTree r] [Fintype M]
+
+lemma finHeight_lt_iff_satisfies_boxbot {i : M} :
+    Frame.World.finHeight i < n ↔ i ⊧ □^[n] ⊥ := by
+  simp only [Frame.finHeight_lt_iff_relItr, Formula.Kripke.Satisfies.multibox_def]
+  simp
+
+lemma finHeight_pos_of_dia {i : M} (hA : i ⊧ ◇ A) : 0 < Frame.World.finHeight i := by
+  have : ∃ j, i ≺ j ∧ j ⊧ A := Formula.Kripke.Satisfies.dia_def.mp hA
+  rcases this with ⟨j, hj, _⟩
+  apply lt_fcwHeight hj (by simp)
+
+@[simp] lemma Model.extendRoot.finHeight₁ :
+    (M.extendRoot 1).finHeight = M.finHeight + 1 := Frame.extendRoot.finHeight₁
+
+end
+
+end Kripke
+
+end
+
+end LO.Modal
