Foundation/Modal/ZeroSubstitution.lean
@@ -1,0 +1,16 @@
+import Foundation.Modal.Letterless
+
+namespace LO.Modal
+
+def ZeroSubstitution (α) := {s : Substitution α // ∀ {a : α}, ((.atom a)⟦s⟧).letterless }
+
+lemma Formula.letterless_zeroSubst {φ : Formula α} {s : ZeroSubstitution α} : (φ⟦s.1⟧).letterless := by
+  induction φ <;> simp [Formula.letterless, *];
+  case hatom => exact s.2;
+
+lemma Formula.toModalFormula.letterless {φ : Propositional.Formula α} (h : φ.letterless) : φ.toModalFormula.letterless := by
+  induction φ using Propositional.Formula.rec' <;> simp_all [Propositional.Formula.letterless, Formula.letterless];
+
+instance : Coe (Propositional.ZeroSubstitution α) (Modal.ZeroSubstitution α) := ⟨λ ⟨s, p⟩ => ⟨λ φ => s φ, λ {_} => Formula.toModalFormula.letterless p⟩⟩
+
+end LO.Modal
