Foundation/Propositional/Logic/PostComplete.lean
@@ -3,14 +3,6 @@ import Foundation.Propositional.Kripke.Logic.Cl
 import Foundation.Propositional.ClassicalSemantics.Hilbert
 import Foundation.Propositional.ClassicalSemantics.ZeroSubst
 
-lemma Set.ssubset_of_subset_ne {α : Type*} {s t : Set α} (h : s ⊆ t) (hne : s ≠ t) : s ⊂ t := by
-  constructor;
-  . assumption;
-  . revert hne;
-    contrapose!;
-    intro _;
-    apply Set.eq_of_subset_of_subset <;> assumption;
-
 namespace LO.Propositional
 
 namespace Logic
