Foundation/ProvabilityLogic/Realization.lean
@@ -3,6 +3,7 @@ import Foundation.FirstOrder.Internal.DerivabilityCondition
 import Foundation.FirstOrder.Incompleteness.Examples
 import Foundation.Logic.HilbertStyle.Cl
 import Foundation.Modal.Hilbert.Normal.Basic
+import Foundation.Modal.Letterless
 
 namespace LO
 
